finished!

InsertionSort.dfy
@@ -1,16 +1,16 @@
 
 method PairInsertionSort(a: array<int>)
-	ensures Sorted1(a,0,a.Length-1)
+	ensures Sorted(a,0,a.Length-1)
 	ensures multiset(a[..]) == multiset(old(a[..]))
 	modifies a
 {
-	//introdue local variable + introduce logical constant + weaken precondition
+	//introduce logical constant + weaken precondition
 	ghost var A := multiset(old(a[..]));
 	PairInsertionSort1(a,A);
 }
 method PairInsertionSort1(a: array<int>, ghost A: multiset<int>) 	
 	requires multiset(a[..])==A
-	ensures Sorted1(a,0,a.Length-1)
+	ensures Sorted(a,0,a.Length-1)
 	ensures multiset(a[..]) == A
 	modifies a
 {
@@ -22,8 +22,7 @@ method PairInsertionSort1(a: array<int>, ghost A: multiset<int>)
 }
 method initIJ(ghost a: array<int>, j0: int,i0:nat, ghost A: multiset<int>) returns (j: int,i:nat)
 	requires multiset(a[..])==A
-	ensures InvPair(a[..],j,i,A)
-	modifies a
+	ensures MainLoopInv(a[..],j,i,A)
 	{
 		j,i:=j0,i0;
 		//assignment
@@ -32,37 +31,25 @@ method initIJ(ghost a: array<int>, j0: int,i0:nat, ghost A: multiset<int>) retur
 	}
 lemma LemmainitIJ( a: array<int>, j: int,i:nat,  A: multiset<int>)
 	requires multiset(a[..])==A
-	ensures InvPair(a[..],-1,0,A)
+	ensures MainLoopInv(a[..],-1,0,A)
 {}
 
 method PairInsertionSort2(a: array<int>, j0: int,i0:nat,x0:int, y0:int, ghost A: multiset<int>) returns (j: int,i:nat,x:int,y:int)
-	requires InvPair(a[..],j0,i0,A)
-	ensures Sorted1(a,0,a.Length-1)
+	requires MainLoopInv(a[..],j0,i0,A)
+	ensures Sorted(a,0,a.Length-1)
 	ensures multiset(a[..]) == A
 	modifies a
 {
-	//sequential composition
+	//sequential composition + contract frame
 	j,i,x,y:=j0,i0,x0,y0;
 	j,i,x,y:=MainLoop(a,j,i,x,y,A);
-	if i==a.Length-1{
-		j,y := i-1,a[i];
-		while j>=0 && a[j] >y
-			invariant Inv4Pair(a[..],j,i,x,y,A)
-			decreases j
-		{
-			SwapPair(a,j+1,j,A);
-			j:=j-1;
-		}
-	}
-	else {
-
-	}	
+	j,y:=PairInsertionSort3(a,j,i,y,A);	
 
 }
 
 method MainLoop(a: array<int>, j0: int,i0:nat,x0:int, y0:int, ghost A: multiset<int>) returns (j: int,i:nat,x:int,y:int)
-	requires InvPair(a[..],j0,i0,A)
-	ensures InvPair(a[..],j,i,A) && !GuardMainLoop(a,i)
+	requires MainLoopInv(a[..],j0,i0,A)
+	ensures MainLoopInv(a[..],j,i,A) && !GuardMainLoop(a,i)
 	modifies a
 
 {
@@ -70,26 +57,26 @@ method MainLoop(a: array<int>, j0: int,i0:nat,x0:int, y0:int, ghost A: multiset<
 	j,i,x,y:=j0,i0,x0,y0;
 	while GuardMainLoop(a,i)
 		decreases a.Length - i
-		invariant InvPair(a[..],j,i,A)
+		invariant MainLoopInv(a[..],j,i,A)
 	{
 		j,i,x,y:=MainLoopBody(a,j,i,x,y,A);
 	}
 }
 
 method MainLoopBody(a: array<int>, j0: int,i0:nat,x0:int, y0:int, ghost A: multiset<int>) returns (j: int,i:nat,x:int,y:int)
-	requires InvPair(a[..],j0,i0,A) && GuardMainLoop(a,i0)
-	ensures InvPair(a[..],j,i,A) && (a.Length-i)< (a.Length-i0)
+	requires MainLoopInv(a[..],j0,i0,A) && GuardMainLoop(a,i0)
+	ensures MainLoopInv(a[..],j,i,A) && (a.Length-i)< (a.Length-i0)
 	modifies a
 {
 	//sequential composition+contract frame
 	j,i,x,y:=j0,i0,x0,y0;
 	j,x,y:=preFirstInnerLoop(a,j,i,x,y,A);
-	j,i,x,y:=MainLoopBody2(a,j,i,x,y,A);
+	j,i:=MainLoopBody2(a,j,i,x,y,A);
 }
 
 method preFirstInnerLoop(a: array<int>, j0: int,i:nat,x0:int, y0:int, ghost A: multiset<int>) returns (j:int,x:int,y:int)
-	requires InvPair(a[..],j0,i,A) && GuardMainLoop(a,i)
-	ensures Inv2Pair(a[..],j,i,x,y,A)
+	requires MainLoopInv(a[..],j0,i,A) && GuardMainLoop(a,i)
+	ensures FirstInnerLoopInv(a[..],j,i,x,y,A)
 	{
 		j,x,y:=j0,x0,y0;
 		//leading assignemnt+following assignment+contract frame+weaken precondition
@@ -97,9 +84,9 @@ method preFirstInnerLoop(a: array<int>, j0: int,i:nat,x0:int, y0:int, ghost A: m
 		x,y:=adjustXY(a,j,i,x,y,A);
 		j:= i-1;
 	}
-method adjustXY(a: array<int>, j: int,i:nat,x0:int, y0:int, ghost A: multiset<int>) returns (x:int,y:int)
-	requires InvPair(a[..],j,i,A) && GuardMainLoop(a,i) && x0==a[i]&&y0==a[i+1]
-	ensures Inv2Pair(a[..],i-1,i,x,y,A)
+method adjustXY(a: array<int>, ghost j: int,ghost i:nat,x0:int, y0:int, ghost A: multiset<int>) returns (x:int,y:int)
+	requires MainLoopInv(a[..],j,i,A) && GuardMainLoop(a,i) && x0==a[i]&&y0==a[i+1]
+	ensures FirstInnerLoopInv(a[..],i-1,i,x,y,A)
 	{
 		x,y:=x0,y0;
 		//alternaion
@@ -110,9 +97,9 @@ method adjustXY(a: array<int>, j: int,i:nat,x0:int, y0:int, ghost A: multiset<in
 			LemmaxGreaterOrEqual(a,j,i,x,y,A);
 		} 
 	}
-method xSmaller (a: array<int>, j: int,i:nat,x0:int, y0:int, ghost A: multiset<int>) returns (x:int,y:int)
-	requires InvPair(a[..],j,i,A) && GuardMainLoop(a,i) && x0==a[i]&&y0==a[i+1] && x0<y0
-	ensures Inv2Pair(a[..],i-1,i,x,y,A)
+method xSmaller (a: array<int>,ghost j: int,ghost i:nat,x0:int, y0:int, ghost A: multiset<int>) returns (x:int,y:int)
+	requires MainLoopInv(a[..],j,i,A) && GuardMainLoop(a,i) && x0==a[i]&&y0==a[i+1] && x0<y0
+	ensures FirstInnerLoopInv(a[..],i-1,i,x,y,A)
 
 	{
 		x,y:=x0,y0;
@@ -121,42 +108,42 @@ method xSmaller (a: array<int>, j: int,i:nat,x0:int, y0:int, ghost A: multiset<i
 	}
 
 lemma LemmaxSmaller (a: array<int>, j: int,i:nat,x:int, y:int,  A: multiset<int>)
-	requires InvPair(a[..],j,i,A) && GuardMainLoop(a,i) && x==a[i]&&y==a[i+1] && x<y
-	ensures Inv2Pair(a[..],i-1,i,y,x,A)
+	requires MainLoopInv(a[..],j,i,A) && GuardMainLoop(a,i) && x==a[i]&&y==a[i+1] && x<y
+	ensures FirstInnerLoopInv(a[..],i-1,i,y,x,A)
 
 lemma LemmaxGreaterOrEqual (a: array<int>, j: int,i:nat,x:int, y:int,  A: multiset<int>)
-	requires InvPair(a[..],j,i,A) && GuardMainLoop(a,i) && x==a[i]&&y==a[i+1] && x>=y
-	ensures Inv2Pair(a[..],i-1,i,x,y,A)
+	requires MainLoopInv(a[..],j,i,A) && GuardMainLoop(a,i) && x==a[i]&&y==a[i+1] && x>=y
+	ensures FirstInnerLoopInv(a[..],i-1,i,x,y,A)
 
-method MainLoopBody2(a: array<int>, j0: int,i0:nat,x0:int, y0:int, ghost A: multiset<int>) returns (j: int,i:nat,x:int,y:int)
-	requires Inv2Pair(a[..],j0,i0,x0,y0,A)
-	ensures InvPair(a[..],j,i,A) && (a.Length-i)< (a.Length-i0)
+method MainLoopBody2(a: array<int>, j0: int,i0:nat,x:int, y:int, ghost A: multiset<int>) returns (j: int,i:nat)
+	requires FirstInnerLoopInv(a[..],j0,i0,x,y,A)
+	ensures MainLoopInv(a[..],j,i,A) && (a.Length-i)< (a.Length-i0)
 	modifies a
 {
 	//sequential composition+contract frame
-	j,i,x,y:=j0,i0,x0,y0;
+	j,i:=j0,i0;
 	j:=firstInnerLoop(a,j,i,x,y,A);
-	j,i,x,y:=MainLoopBody3(a,j,i,x,y,A);
+	j,i:=MainLoopBody3(a,j,i,x,y,A);
 }
 
-method firstInnerLoop(a: array<int>, j0: int,i:nat,x:int, y:int, ghost A: multiset<int>) returns (j: int)
-	requires Inv2Pair(a[..],j0,i,x,y,A)
-	ensures Inv2Pair(a[..],j,i,x,y,A) && !GuardSecondLoop(a,j,x)
+method firstInnerLoop(a: array<int>, j0: int,ghost i:nat,x:int,ghost y:int, ghost A: multiset<int>) returns (j: int)
+	requires FirstInnerLoopInv(a[..],j0,i,x,y,A)
+	ensures FirstInnerLoopInv(a[..],j,i,x,y,A) && !GuardFirstInnerLoop(a,j,x)
 	modifies a
 	{
 		j:=j0;
 		//iteration
-		while GuardSecondLoop(a,j,x)
-		invariant Inv2Pair(a[..],j,i,x,y,A)
+		while GuardFirstInnerLoop(a,j,x)
+		invariant FirstInnerLoopInv(a[..],j,i,x,y,A)
 		decreases j
 		{
 			j:=firstInnerLoopBody(a,j,i,x,y,A);
 		}
 	}
 
-method firstInnerLoopBody(a: array<int>, j0: int,i:nat,x:int, y:int, ghost A: multiset<int>) returns (j: int)
-	requires Inv2Pair(a[..],j0,i,x,y,A) && GuardSecondLoop(a,j0,x)
-	ensures Inv2Pair(a[..],j,i,x,y,A) && j<j0
+method firstInnerLoopBody(a: array<int>, j0: int,ghost i:nat,ghost x:int,ghost y:int, ghost A: multiset<int>) returns (j: int)
+	requires FirstInnerLoopInv(a[..],j0,i,x,y,A) && GuardFirstInnerLoop(a,j0,x)
+	ensures FirstInnerLoopInv(a[..],j,i,x,y,A) && j<j0
 	modifies a
 
 	{
@@ -165,9 +152,9 @@ method firstInnerLoopBody(a: array<int>, j0: int,i:nat,x:int, y:int, ghost A: mu
 		SwapFirstInner(a,j,i,x,y,A);
 		j:=j-1;
 	}
-method {:verify true} SwapFirstInner(a: array<int>, j:int, i: nat,x:int,y:int ,ghost A: multiset<int>) 
-	requires Inv2Pair(a[..], j, i,x, y, A) && GuardSecondLoop(a,j,x)
-	ensures Inv2Pair(a[..], j-1, i,x, y, A) // && j-1 < j
+method {:verify true} SwapFirstInner(a: array<int>, j:int,ghost i: nat,ghost x:int,ghost y:int ,ghost A: multiset<int>) 
+	requires FirstInnerLoopInv(a[..], j, i,x, y, A) && GuardFirstInnerLoop(a,j,x)
+	ensures FirstInnerLoopInv(a[..], j-1, i,x, y, A) && j-1 < j
 	modifies a
 {
 	// assignment
@@ -176,98 +163,278 @@ method {:verify true} SwapFirstInner(a: array<int>, j:int, i: nat,x:int,y:int ,g
 }
 
 lemma LemmaSwapFirstInner(a: array<int>, j: int, i: nat,x:int,y:int, A: multiset<int>)
-	requires Inv2Pair(a[..], j, i, x, y, A) && GuardSecondLoop(a,j,x)
-	ensures Inv2Pair(a[..][j := a[j+2]][j+2 := a[j]], j-1, i, x, y, A) 
+	requires FirstInnerLoopInv(a[..], j, i, x, y, A) && GuardFirstInnerLoop(a,j,x)
+	ensures FirstInnerLoopInv(a[..][j := a[j+2]][j+2 := a[j]], j-1, i, x, y, A) 
 {}
 
-method MainLoopBody3(a: array<int>, j0: int,i0:nat,x0:int, y0:int, ghost A: multiset<int>) returns (j: int,i:nat,x:int,y:int)
-	requires Inv2Pair(a[..],j0,i0,x0,y0,A) && !GuardSecondLoop(a,j0,x0)
-	ensures InvPair(a[..],j,i,A) && (a.Length-i)< (a.Length-i0)
+method MainLoopBody3(a: array<int>, j0: int,i0:nat,x:int, y:int, ghost A: multiset<int>) returns (j: int,i:nat)
+	requires FirstInnerLoopInv(a[..],j0,i0,x,y,A) && !GuardFirstInnerLoop(a,j0,x)
+	ensures MainLoopInv(a[..],j,i,A) && (a.Length-i)< (a.Length-i0)
 	modifies a
-	{
-		j,i,x,y:=j0,i0,x0,y0;
-		if a[j+2]!=x{
-		SwapPair(a,j+2,j+1,A);
+{
+	//sequential composition+contract frame 
+	j,i:=j0,i0;
+	preSecondInnerLoop(a,j,i,x,y,A);
+	j,i:=MainLoopBody4(a,j,i,y,A);
+}
+
+method preSecondInnerLoop(a: array<int>, j: int,ghost i:nat,x:int, ghost y:int, ghost A: multiset<int>)
+	requires FirstInnerLoopInv(a[..],j,i,x,y,A) && !GuardFirstInnerLoop(a,j,x)
+	ensures SecondInnerLoopInv(a[..],j,i,y,A)
+	modifies a
+{
+	//alternation
+	if a[j+2]!=x{
+		SwapPreSecondInner(a,j,i,x,y,A);
 	}	
 	else{
-		LemmaMidNoswap(a[..],j,i,x,y,A);
+		LemmaPreSecondInnerNoswap(a,j,i,x,y,A);
 	}
-	
-	
-	while j>=0 && a[j] > y
-		invariant Inv3Pair(a[..],j,i,x,y,A)
+}
+
+method {:verify true} SwapPreSecondInner(a: array<int>, j:int,ghost i: nat,ghost x:int,ghost y:int ,ghost A: multiset<int>) 
+	requires FirstInnerLoopInv(a[..],j,i,x,y,A) && !GuardFirstInnerLoop(a,j,x) && a[j+2]!=x
+	ensures SecondInnerLoopInv(a[..],j,i,y,A)
+	modifies a
+{
+	// assignment
+	LemmaSwapPreSecondInner(a, j, i, x, y, A);
+	a[j+2], a[j+1] := a[j+1], a[j+2];
+}
+
+lemma LemmaSwapPreSecondInner(a: array<int>, j: int, i: nat,x:int,y:int, A: multiset<int>)
+	requires FirstInnerLoopInv(a[..],j,i,x,y,A) && !GuardFirstInnerLoop(a,j,x) && a[j+2]!=x
+	ensures SecondInnerLoopInv(a[..][j+1 := a[j+2]][j+2 := a[j+1]], j, i, y, A) 
+{}
+
+lemma LemmaPreSecondInnerNoswap(a: array<int>,j:int,i:nat,x:int,y:int, A: multiset<int>)
+	requires FirstInnerLoopInv(a[..],j,i,x,y,A) && !GuardFirstInnerLoop(a,j,x) && a[j+2]==x
+	ensures SecondInnerLoopInv(a[..],j,i,y,A)
+{
+}
+
+method MainLoopBody4(a: array<int>, j0: int,i0:nat, y:int, ghost A: multiset<int>) returns (j: int,i:nat)
+	requires SecondInnerLoopInv(a[..],j0,i0,y,A)
+	ensures MainLoopInv(a[..],j,i,A) && (a.Length-i)< (a.Length-i0)
+	modifies a
+{
+	//sequential composition + contract frame
+	j,i:=j0,i0;
+	j:=SecondInnerLoop(a,j,i,y,A);
+	i:=MainLoopBody5(a,j,i,y,A);	
+}
+method SecondInnerLoop(a: array<int>, j0: int,ghost i:nat,y:int, ghost A: multiset<int>) returns (j: int)
+	requires SecondInnerLoopInv(a[..],j0,i,y,A)
+	ensures SecondInnerLoopInv(a[..],j,i,y,A) && !GuardSecondInnerLoop(a,j,y)
+	modifies a
+{
+	//iteration
+	j:=j0;
+	while GuardSecondInnerLoop(a,j,y)
+		invariant SecondInnerLoopInv(a[..],j,i,y,A)
 		decreases j
 		{
-			SwapPair(a,j+1,j,A);
-			j:=j-1;
+			j:=SecondInnerLoopBody(a,j,i,y,A);
 		}
-	
-	i:=i+2;	
+}
+method SecondInnerLoopBody(a: array<int>, j0: int,ghost i:nat,y:int, ghost A: multiset<int>) returns (j: int)
+	requires SecondInnerLoopInv(a[..],j0,i,y,A) && GuardSecondInnerLoop(a,j0,y)
+	ensures SecondInnerLoopInv(a[..],j,i,y,A) && j<j0
+	modifies a
+{
+	j:=j0;
+	//contract frame+ following assignment
+	SwapSecondInner(a,j,i,y,A);
+	j:=j-1;
+}
+
+method {:verify true} SwapSecondInner(a: array<int>, j:int,ghost i: nat,ghost y:int ,ghost A: multiset<int>) 
+	requires SecondInnerLoopInv(a[..],j,i,y,A) && GuardSecondInnerLoop(a,j,y)
+	ensures SecondInnerLoopInv(a[..],j-1,i,y,A) && j-1<j
+	modifies a
+{
+	// assignment
+	LemmaSwapSecondInner(a, j, i, y, A);
+	a[j+1], a[j] := a[j], a[j+1];
+}
+
+lemma LemmaSwapSecondInner(a: array<int>, j: int, i: nat,y:int, A: multiset<int>)
+	requires SecondInnerLoopInv(a[..],j,i,y,A) && GuardSecondInnerLoop(a,j,y)
+	ensures SecondInnerLoopInv(a[..][j := a[j+1]][j+1 := a[j]], j-1, i, y, A) && j-1<j
+{}
+
+method MainLoopBody5(a: array<int>, j: int,i0:nat, ghost y:int, ghost A: multiset<int>) returns (i:nat)
+	requires SecondInnerLoopInv(a[..],j,i0,y,A) && !GuardSecondInnerLoop(a,j,y)
+	ensures MainLoopInv(a[..],j,i,A) && (a.Length-i)< (a.Length-i0)
+{
+	i:=i0;
+	//assignment
+	LemmaMainLoopBody5(a,j,i,y,A);
+	i:=i+2;
+}
+
+lemma LemmaMainLoopBody5(a: array<int>, j: int,i:nat,  y:int,  A: multiset<int>) 
+	requires SecondInnerLoopInv(a[..],j,i,y,A) && !GuardSecondInnerLoop(a,j,y)
+	ensures MainLoopInv(a[..],j,i+2,A) && (a.Length-(i+2))< (a.Length-i)
+	{}
+
+
+method PairInsertionSort3(a: array<int>, j0: int,i:nat, y0:int, ghost A: multiset<int>) returns (j: int,y:int)
+	requires  MainLoopInv(a[..],j0,i,A) && !GuardMainLoop(a,i)
+	ensures Sorted(a,0,a.Length-1)
+	ensures multiset(a[..]) == A
+	modifies a
+{
+	j,y:=j0,y0;
+	//alternation
+	if i==a.Length-1{
+		j,y:=iEqualsLastPlace(a,j,i,y,A);
 	}
+	else {
+		LemmaINotEqualsLastPlace(a,j,i,y,A);
+	}	
+}
+lemma LemmaINotEqualsLastPlace(a: array<int>, j: int,i:nat, y:int,  A: multiset<int>)
+	requires MainLoopInv(a[..],j,i,A) && !GuardMainLoop(a,i) && i!=a.Length-1
+	ensures Sorted(a,0,a.Length-1)
+	ensures multiset(a[..]) == A
+	{}
+	
+method iEqualsLastPlace(a: array<int>, j0: int,i:nat, y0:int, ghost A: multiset<int>) returns (j: int,y:int)
+	requires MainLoopInv(a[..],j0,i,A) && !GuardMainLoop(a,i) && i==a.Length-1
+	ensures Sorted(a,0,a.Length-1)
+	ensures multiset(a[..]) == A
+	modifies a
+{
+	j,y:=j0,y0;
+	//sequential composition + strengthen postcondition+contract frame
+	j,y := initJI(a,j,i,y,A);
+	j:=postLoop(a,j,i,y,A);
+	LemmaStrenghtenPostLoop(a,j,i,y,A);
+}
+lemma LemmaStrenghtenPostLoop(a: array<int>, j: int,i:nat, y:int,  A: multiset<int>) 
+	requires PostLoopInv(a[..],j,i,y,A)&& !GuardPostLoop(a,j,y)
+	ensures Sorted(a,0,a.Length-1)
+	ensures multiset(a[..]) == A
+
+method initJI(a: array<int>, j0: int,i:nat, y0:int, ghost A: multiset<int>) returns (j: int,y:int)
+	requires MainLoopInv(a[..],j0,i,A) && !GuardMainLoop(a,i) && i==a.Length-1
+	ensures PostLoopInv(a[..],j,i,y,A)
+{
+	j,y:=j0,y0;
+	//assignment
+	j,y := i-1,a[i];
+}
+
+lemma LemmainitJI(a: array<int>, j0: int,i:nat, y0:int,  A: multiset<int>) 
+	requires MainLoopInv(a[..],j0,i,A) && !GuardMainLoop(a,i) && i==a.Length-1
+	ensures PostLoopInv(a[..],i-1,i,a[i],A)
+	{}
+
+method postLoop(a: array<int>, j0: int,i:nat, y:int, ghost A: multiset<int>) returns (j: int)
+	requires PostLoopInv(a[..],j0,i,y,A)
+	ensures PostLoopInv(a[..],j,i,y,A)&& !GuardPostLoop(a,j,y)
+	modifies a
+{
+	j:=j0;
+	//iteration
+	while GuardPostLoop(a,j,y)
+		invariant PostLoopInv(a[..],j,i,y,A)
+		decreases j
+	{
+		j:=postLoopBody(a,j,i,y,A);
+	}
+}
+
+method postLoopBody(a: array<int>, j0: int,i:nat, y:int, ghost A: multiset<int>) returns (j: int)
+	requires PostLoopInv(a[..],j0,i,y,A) && GuardPostLoop(a,j0,y)
+	ensures PostLoopInv(a[..],j,i,y,A)&& j<j0
+	modifies a
+{
+	j:=j0;
+	//following assignment+contract frame
+	SwapPost(a,j,i,y,A);
+	j:=j-1;
+}
+
+method {:verify true} SwapPost(a: array<int>, j:int,ghost i: nat,ghost y:int ,ghost A: multiset<int>) 
+	requires PostLoopInv(a[..],j,i,y,A) && GuardPostLoop(a,j,y)
+	ensures PostLoopInv(a[..],j-1,i,y,A)&& j-1<j
+	modifies a
+{
+	// assignment
+	LemmaSwapPost(a, j, i, y, A);
+	a[j+1], a[j] := a[j], a[j+1];
+}
+
+lemma LemmaSwapPost(a: array<int>, j: int, i: nat,y:int, A: multiset<int>)
+	requires PostLoopInv(a[..],j,i,y,A) && GuardPostLoop(a,j,y)
+	ensures PostLoopInv(a[..][j := a[j+1]][j+1 := a[j]], j-1, i, y, A) && j-1<j
+{}
 predicate method GuardMainLoop(a: array<int>,i:nat)
 {
 	i < a.Length-1	
 }
 
-predicate method GuardSecondLoop(a: array<int>,j:int,x:int)
+predicate method GuardFirstInnerLoop(a: array<int>,j:int,x:int)
 	requires -1<=j<=a.Length-3
 	reads a
 {
 	 j>=0 && a[j]>x	
 }
 
-
-lemma LemmaMidswap(a: seq<int>,j:int,i:nat,x:int,y:int, A: multiset<int>)
-	requires Inv2Pair(a,j,i,x,y,A)
-	requires j<0 || a[j]<=x
-	requires a[j+2]!=x
-	ensures Inv3Pair(a[j+1:=a[j+2]][j+2:=a[j+1]],j,i,x,y,A)
+predicate method GuardSecondInnerLoop(a: array<int>,j:int,y:int)
+	requires -1<=j<=a.Length-3
+	reads a
 {
+	 j>=0 && a[j] > y
 }
 
-lemma LemmaMidNoswap(a: seq<int>,j:int,i:nat,x:int,y:int, A: multiset<int>)
-	requires Inv2Pair(a,j,i,x,y,A)
-	requires j<0 || a[j]<=x
-	requires a[j+2]==x
-	ensures Inv3Pair(a,j,i,x,y,A)
+predicate method GuardPostLoop(a: array<int>,j:int,y:int)
+	requires -1<=j<=a.Length-2
+	reads a
 {
+	 j>=0 && a[j] > y
 }
-predicate InvPair(a: seq<int>, j: int, i:nat, A: multiset<int>)
+
+
+
+predicate MainLoopInv(a: seq<int>, j: int, i:nat, A: multiset<int>)
 {
 	0<=i<=|a| &&
 	(|a|>1 ==> (-1<=j<=|a|-3)) &&
-	SortedSequence1(a,0,i-1) &&
+	SortedSequence(a,0,i-1) &&
 	multiset(a)==A
 }
-predicate Inv2Pair(a: seq<int>, j: int,i:nat,x:int, y:int, A: multiset<int>)
+predicate FirstInnerLoopInv(a: seq<int>, j: int,i:nat,x:int, y:int, A: multiset<int>)
 {
 	0<=i<=|a|-2 &&
 	-1<=j<=|a|-3 &&
-	SortedSequence1(a,0,j)&&
-	SortedSequence1(a,j+2,i+1)&&
+	SortedSequence(a,0,j)&&
+	SortedSequence(a,j+2,i+1)&&
 	(0<=j<i-1 ==> a[j+3]>=a[j]) &&
 	(j<i-1  ==> a[j+3]>x) &&
 	((x==a[j+1]&&y==a[j+2]) || (x==a[j+2]&&y==a[j+1])) && x>=y &&
 	multiset(a)==A
 }
 
-predicate Inv3Pair(a: seq<int>, j: int,i:nat,x:int, y:int, A: multiset<int>)
+predicate SecondInnerLoopInv(a: seq<int>, j: int,i:nat, y:int, A: multiset<int>)
 {
 	0<=i<=|a|-2 &&
 	-1<=j<=|a|-3 &&
-	SortedSequence1(a,0,j)&&
-	SortedSequence1(a,j+1,i+1)&&
+	SortedSequence(a,0,j)&&
+	SortedSequence(a,j+1,i+1)&&
 	a[j+2]>=y &&
 	(j>=0 ==> a[j+2]>=a[j]) &&
 	a[j+1]==y &&
 	multiset(a)==A
 }
 
-predicate Inv4Pair(a: seq<int>, j: int,i:nat,x:int, y:int, A: multiset<int>)
+predicate PostLoopInv(a: seq<int>, j: int,i:nat, y:int, A: multiset<int>)
 {
 	-1<=j<=|a|-2&&
-	SortedSequence1(a,0,j)&&
-	SortedSequence1(a,j+1,|a|-1)&&
+	SortedSequence(a,0,j)&&
+	SortedSequence(a,j+1,|a|-1)&&
 	a[j+1]==y && 
 	(j<=|a|-3 ==> a[j+2]>y) &&
 	(0<=j<=|a|-3 ==> a[j+2]>=a[j]) &&
@@ -276,69 +443,15 @@ predicate Inv4Pair(a: seq<int>, j: int,i:nat,x:int, y:int, A: multiset<int>)
 
 
 
-predicate Sorted1(a: array<int>, i:nat, j:int)
+predicate Sorted(a: array<int>, i:nat, j:int)
 	requires i<=j ==> (0<=i<a.Length && 0<=j<a.Length)
 	reads a
 {
 	 (forall k :: i <= k < j-1 ==> a[k] <= a[k+1]) 
 }
 
-predicate SortedSequence1(a: seq<int>, i:nat, h:int)
+predicate SortedSequence(a: seq<int>, i:nat, h:int)
 	requires i<=h ==> (0<=i <|a| && 0<=h<|a|)
 {
 	(forall k :: i <=  k <= h-1 ==> a[k] <= a[k+1])
 }
-
-method {:verify true} SwapPair(a: array<int>, x:nat,y:nat,ghost A: multiset<int>)
-	requires multiset(a[..]) == A
-	requires 0<=x<a.Length && 0<=y<a.Length
-	requires x!=y
-	ensures multiset(a[..]) == A
-	ensures a[x] == old(a[y])
-	ensures a[y] == old(a[x])
-	ensures forall i :: 0<=i<a.Length ==> ((i!=x && i!=y) ==> a[i]==old(a[i]))
-	modifies a
-{
-	// assignment
-	LemmaSwapPair(a[..],old(a[..]), x, y, A);
-	a[x], a[y] := a[y], a[x];
-}
-
-lemma LemmaSwapPair(a: seq<int>,oldA :seq <int>, x: nat, y: nat, A: multiset<int>)
-	requires a==oldA
-	requires multiset(a[..]) == A
-	requires 0<=x<|a| && 0<=y<|a|
-	requires x!=y
-	ensures multiset(a[x:= oldA[y]][y:=oldA[x]]) == A
-	ensures a[x:= oldA[y]][y:=oldA[x]][x] == oldA[y]
-	ensures  a[x:= oldA[y]][y:=oldA[x]][y] == oldA[x]
-	ensures forall i :: 0<=i<|a| ==> ((i!=x && i!=y) ==> a[x:= oldA[y]][y:=oldA[x]][i]==oldA[i])
-{}
-
-/*method {:verify true} SwapPair1(a: array<int>, x:nat,y:nat,i:nat,ghost A: multiset<int>)
-	requires multiset(a[..]) == A
-	requires 0<=x<a.Length && 0<=y<a.Length
-	requires 0<=i<=a.Length-2
-	requires SortedSequence1(a[..],0,x)&& SortedSequence1(a[..],y,i)
-	ensures multiset(a[..]) == A
-	ensures SortedSequence1(a[..],0,x) && SortedSequence1(a[..],y,i)
-	ensures 0<=i<=a.Length-2
-	modifies a
-{
-	// assignment
-	//LemmaSwapPair1(a[..],old(a[..]), x, y, A);
-	a[x], a[y] := a[y], a[x];
-}
-
-lemma LemmaSwapPair1(a: seq<int>,oldA :seq <int>, x: nat, y: nat, A: multiset<int>)
-	requires a==oldA
-	requires multiset(a[..]) == A
-	requires 0<=x<|a| && 0<=y<|a|
-	requires x!=y
-	ensures multiset(a[x:= oldA[y]][y:=oldA[x]]) == A
-	ensures a[x:= oldA[y]][y:=oldA[x]][x] == oldA[y]
-	ensures  a[x:= oldA[y]][y:=oldA[x]][y] == oldA[x]
-	ensures forall i :: 0<=i<|a| ==> ((i!=x && i!=y) ==> a[x:= oldA[y]][y:=oldA[x]][i]==oldA[i])
-{}
-
-*/
